daily save 29/03

meta-theory/pure_demandScript.sml
@@ -7,10 +7,910 @@ open arithmeticTheory listTheory stringTheory alistTheory dep_rewrite
      optionTheory pairTheory ltreeTheory llistTheory bagTheory
      BasicProvers pred_setTheory relationTheory rich_listTheory finite_mapTheory;
 open pure_expTheory pure_valueTheory pure_evalTheory pure_eval_lemmasTheory
-     pure_exp_lemmasTheory pure_miscTheory pure_exp_relTheory pure_congruenceTheory;
-open  pure_alpha_equivTheory pure_exp_eq_in_ctxtTheory;
+     pure_exp_lemmasTheory pure_miscTheory pure_exp_relTheory pure_congruenceTheory
+     pure_alpha_equivTheory pure_exp_eq_in_ctxtTheory pure_alpha_equivTheory;
 
 val _ = new_theory "pure_demand";
+
+(** begin ctxt **)
+
+(* Definitions *)
+
+Datatype:
+  ctxt = Nil
+       | IsFree string ctxt
+       | Bind string exp ctxt
+       | RecBind ((string # exp) list) ctxt
+End
+
+Definition exp_eq_in_ctxt_def:
+  exp_eq_in_ctxt Nil = (λe1 e2. e1 ≈ e2) ∧
+  exp_eq_in_ctxt (IsFree s c) e1 e2 = (∀e3. closed e3 ⇒ exp_eq_in_ctxt c (Let s e3 e1) (Let s e3 e2)) ∧
+  exp_eq_in_ctxt (Bind s e3 c) e1 e2 = exp_eq_in_ctxt c (Let s e3 e1) (Let s e3 e2) ∧
+  exp_eq_in_ctxt (RecBind l c) e1 e2 = exp_eq_in_ctxt c (Letrec l e1) (Letrec l e2)
+End
+
+Definition ctxt_size_def:
+  ctxt_size Nil = 0n ∧
+  ctxt_size (IsFree s ctxt) = 1 + ctxt_size ctxt ∧
+  ctxt_size (Bind s e ctxt) = 1 + list_size char_size s +  exp_size e + ctxt_size ctxt ∧
+  ctxt_size (RecBind sel ctxt) = 1 + exp1_size sel + ctxt_size ctxt
+End
+
+(* Preliminaries *)
+
+Theorem exp_eq_l_refl:
+  ∀b l. LIST_REL (λx y. (x ≅? y) b) l l
+Proof
+  gen_tac
+  \\ Induct
+  \\ fs [exp_eq_refl]
+QED
+
+Theorem exp_eq_Apps_cong:
+  ∀l l' b e e'. LIST_REL (λx y. (x ≅? y) b) l l' ⇒ (e ≅? e') b ⇒ (Apps e l ≅? Apps e' l') b
+Proof
+  Induct
+  \\ fs [Apps_def]
+  \\ rw [Apps_def]
+  \\ fs [Apps_def]
+  \\ first_x_assum $ irule
+  \\ fs [exp_eq_App_cong]
+QED
+
+Theorem exp_eq_Lams_cong:
+  ∀l e e' b. (e ≅? e') b ⇒ (Lams l e ≅? Lams l e') b
+Proof
+  Induct
+  \\ rw [Lams_def]
+  \\ fs [exp_eq_Lam_cong]
+QED
+
+Theorem eval_Prim:
+  ∀ope eL eL'. LIST_REL (λe1 e2. eval e1 = eval e2) eL eL' ⇒ eval (Prim ope eL) = eval (Prim ope eL')
+Proof
+  Cases
+  \\ rw [eval_thm]
+  >~[‘MAP _ _ = MAP _ _’]
+  >- (irule LIST_EQ
+      \\ gvs [LIST_REL_EL_EQN, EL_MAP])
+  >~[‘AtomOp’]
+  >- (fs [eval_def]
+      \\ once_rewrite_tac [v_unfold]
+      \\ fs [eval_wh_Prim]
+      \\ qsuff_tac ‘get_atoms (MAP eval_wh eL') = get_atoms (MAP eval_wh eL)’
+      >- (CASE_TAC \\ fs [])
+      \\ fs [get_atoms_def]
+      \\ qsuff_tac ‘EXISTS error_Atom (MAP eval_wh eL) ⇔ EXISTS error_Atom (MAP eval_wh eL')’
+      >- (strip_tac
+          \\ IF_CASES_TAC
+          \\ simp []
+          \\ qsuff_tac ‘MEM wh_Diverge (MAP eval_wh eL) ⇔ MEM wh_Diverge (MAP eval_wh eL')’
+          >- (strip_tac
+              \\ IF_CASES_TAC
+              \\ simp []
+              \\ irule LIST_EQ
+              \\ rw []
+              \\ gvs [LIST_REL_EL_EQN, EL_MAP, EVERY_EL]
+              \\ rpt $ first_x_assum drule
+              \\ once_rewrite_tac [v_unfold]
+              \\ rpt FULL_CASE_TAC
+              \\ rw [dest_Atom_def, error_Atom_def])
+          \\ eq_tac
+          \\ strip_tac
+          \\ gvs [MEM_EL, LIST_REL_EL_EQN]
+          \\ first_assum $ irule_at Any
+          \\ first_assum drule
+          \\ once_rewrite_tac [v_unfold]
+          \\ rpt FULL_CASE_TAC
+          \\ gvs [EL_MAP])
+      \\ eq_tac
+      \\ strip_tac
+      \\ gvs [EXISTS_MEM, MEM_EL, EL_MAP, LIST_REL_EL_EQN]
+      \\ rename1 ‘MAP eval_wh eL2’
+      \\ qexists_tac ‘eval_wh (EL n eL2)’
+      \\ first_x_assum drule
+      \\ once_rewrite_tac [v_unfold]
+      \\ rpt FULL_CASE_TAC
+      \\ fs [error_Atom_def]
+      \\ rw []
+      \\ first_assum $ irule_at Any
+      \\ fs [EL_MAP])
+  \\ Cases_on ‘eL’ \\ Cases_on ‘eL'’ \\ fs []
+  \\ rename1 ‘LIST_REL _ t1 t2’
+  \\ Cases_on ‘t1’ \\ Cases_on ‘t2’ \\ gvs [eval_thm]
+  >~[‘Prim Seq (_::_::_)’]
+  >- (rename1 ‘LIST_REL _ t1 t2’
+      \\ Cases_on ‘t1’ \\ Cases_on ‘t2’
+      \\ gvs [eval_thm, eval_def]
+      \\ once_rewrite_tac [v_unfold]
+      \\ fs [eval_wh_Prim])
+  >~[‘Prim If (_::_::_)’]
+  >- (rename1 ‘LIST_REL _ t1 t2’
+      \\ Cases_on ‘t1’ \\ Cases_on ‘t2’ \\ gvs []
+      >~[‘_::_::_::_’]
+      >- (rename1 ‘LIST_REL _ t1 t2’
+          \\ Cases_on ‘t1’ \\ Cases_on ‘t2’
+          \\ gvs [eval_thm, eval_def]
+          \\ once_rewrite_tac [v_unfold]
+          \\ rw [eval_wh_Prim])
+      \\ rw [eval_def]
+      \\ once_rewrite_tac [v_unfold]
+      \\ rw [eval_wh_Prim])
+  \\ rw [eval_def]
+  \\ once_rewrite_tac [v_unfold]
+  \\ rw [eval_wh_Prim]
+QED
+
+Theorem FLOOKUP_LUPDATE:
+  ∀l f n v. FLOOKUP (f |++ l) n = SOME v ⇒ MEM (n, v) l ∨ FLOOKUP f n = SOME v
+Proof
+  Induct
+  \\ fs [FUPDATE_LIST_THM]
+  \\ PairCases \\ rw []
+  \\ first_x_assum $ dxrule_then assume_tac
+  \\ gvs [FLOOKUP_UPDATE]
+  \\ FULL_CASE_TAC \\ fs []
+QED
+
+Theorem Letrec_Prim:
+  ∀l ope eL b. (Letrec l (Prim ope eL) ≅? Prim ope (MAP (Letrec l) eL)) b
+Proof
+  rw []
+  \\ irule eval_IMP_exp_eq
+  \\ rw [subst_def, eval_thm, subst_funs_def, bind_def]
+  >- (irule eval_Prim
+      \\ rw [LIST_REL_EL_EQN, EL_MAP, subst_def, eval_thm, subst_funs_def]
+      \\ gvs [bind_def]
+      \\ IF_CASES_TAC \\ fs []
+      \\ first_x_assum dxrule
+      \\ strip_tac
+      \\ fs [])
+  \\ fs [MAP_MAP_o]
+  \\ dxrule_then assume_tac FLOOKUP_LUPDATE
+  \\ gvs [FLOOKUP_EMPTY, MEM_EL, EL_MAP]
+  \\ qsuff_tac ‘F’ \\ fs []
+  \\ first_x_assum irule
+  \\ rename1 ‘EL k l’
+  \\ qabbrev_tac ‘p = EL k l’
+  \\ PairCases_on ‘p’
+  \\ gvs [EVERY_EL, EL_MAP]
+  \\ rw []
+  \\ rename1 ‘EL k2 l’
+  \\ qabbrev_tac ‘p' = EL k2 l’
+  \\ PairCases_on ‘p'’
+  \\ gvs []
+  \\ ‘∀v. v ∈ FRANGE (FDIFF f (set (MAP FST l))) ⇒ closed v’
+    by (rw []
+        \\ first_x_assum irule
+        \\ gvs [FRANGE_FLOOKUP, FLOOKUP_FDIFF]
+        \\ pop_assum $ irule_at Any)
+  \\ gvs [freevars_subst, SUBSET_DEF, IN_DIFF, FDOM_FDIFF]
+  \\ rw [MEM_EL]
+  >>~[‘EL _ (MAP FST _) = EL _ (MAP FST _)’]
+  >- (first_assum $ irule_at Any
+      \\ gvs [EL_MAP]
+      \\ rename1 ‘FST p = FST _’
+      \\ PairCases_on ‘p’
+      \\ fs [])
+  >- (first_assum $ irule_at Any
+      \\ gvs [EL_MAP]
+      \\ rename1 ‘FST p = FST _’
+      \\ PairCases_on ‘p’
+      \\ fs [])
+  \\ first_x_assum $ qspecl_then [‘x’] assume_tac
+  \\ pop_assum kall_tac
+  \\ first_x_assum $ qspecl_then [‘x’] assume_tac
+  \\ gvs [] >>~[‘MEM x (MAP FST l)’]
+  >- (gvs [MEM_EL]
+      \\ first_assum $ irule_at Any
+      \\ fs [EL_MAP]
+      \\ rename1 ‘FST p = FST _’
+      \\ PairCases_on ‘p’ \\ fs [])
+  >- (gvs [MEM_EL]
+      \\ first_assum $ irule_at Any
+      \\ fs [EL_MAP]
+      \\ rename1 ‘FST p = FST _’
+      \\ PairCases_on ‘p’ \\ fs [])
+  \\ first_x_assum $ qspecl_then [‘freevars p'1’] assume_tac
+  \\ gvs [MEM_MAP]
+  \\ pop_assum $ qspecl_then [‘EL k2 l’] assume_tac
+  \\ gvs [EL_MEM]
+QED
+
+Theorem Let_Lam:
+  ∀v w e1 e2 b. closed e1 ∧ v ≠ w ⇒ (Let v e1 (Lam w e2) ≅? Lam w (Let v e1 e2)) b
+Proof
+  rw []
+  \\ irule exp_eq_trans
+  \\ irule_at Any beta_equality
+  \\ gvs [subst1_def]
+  \\ irule exp_eq_Lam_cong
+  \\ irule $ iffLR exp_eq_sym
+  \\ irule beta_equality
+  \\ gvs []
+QED
+
+Theorem Let_Lam_weak:
+  ∀v w e1 e2 b. v ≠ w ⇒ w ∉ freevars e1 ⇒ (Let v e1 (Lam w e2) ≅? Lam w (Let v e1 e2)) b
+Proof
+  rw [exp_eq_def, bind_def] >> IF_CASES_TAC >>
+  gvs [app_bisimilarity_eq, exp_eq_refl] >>
+  rpt (irule_at Any IMP_closed_subst) >>
+  drule_then assume_tac $ GSYM subst_fdomsub >>
+  gvs [subst_def, DOMSUB_COMMUTES] >>
+  irule_at Any Let_Lam >>
+  irule_at Any IMP_closed_subst >>
+  rw [FRANGE_FLOOKUP]
+QED
+
+Theorem FDIFF_DOMSUB:
+  ∀f v s. FDIFF (f \\ s) v = (FDIFF f v) \\ s
+Proof
+  rw [FDIFF_def, fmap_domsub, INTER_COMM]
+QED
+
+Theorem MAP_subst_fdomsub:
+  ∀v l f. EVERY (λe. v ∉ freevars e) (MAP SND l) ⇒
+          MAP (λ(s, e). (s, subst (FDIFF f (set (MAP FST l)) \\ v) e)) l
+          = MAP (λ(s, e). (s, subst (FDIFF f (set (MAP FST l))) e)) l
+Proof
+  rw [EVERY_EL] >> irule LIST_EQ >>
+  rw [EL_MAP] >> first_x_assum $ drule_then assume_tac >>
+  rename1 ‘EL x l’ >> qabbrev_tac ‘p = EL x l’ >> PairCases_on ‘p’ >>
+  gvs [subst_fdomsub, EL_MAP]
+QED
+
+Theorem Letrec_Lam:
+  ∀l w e b. EVERY (λe. freevars e ⊆ set (MAP FST l)) (MAP SND l) ∧ ¬MEM w (MAP FST l)
+          ⇒ (Letrec l (Lam w e) ≅? Lam w (Letrec l e)) b
+Proof
+  rw []
+  \\ irule exp_eq_trans
+  \\ irule_at Any beta_equality_Letrec
+  \\ gvs [subst_funs_eq_subst, subst_def]
+  \\ irule exp_eq_Lam_cong
+  \\ irule $ iffLR exp_eq_sym
+  \\ irule exp_eq_trans
+  \\ irule_at Any beta_equality_Letrec
+  \\ gvs [subst_funs_eq_subst]
+  \\ irule eval_IMP_exp_eq
+  \\ rw []
+  \\ rpt AP_TERM_TAC \\ AP_THM_TAC \\ AP_TERM_TAC
+  \\ irule $ GSYM DOMSUB_NOT_IN_DOM
+  \\ gvs [FDOM_FUPDATE_LIST]
+  \\ strip_tac \\ last_x_assum irule
+  \\ gvs [MEM_EL]
+  \\ first_assum $ irule_at Any
+  \\ gvs [EL_MAP]
+  \\ rename1 ‘FST (_ p)’
+  \\ PairCases_on ‘p’
+  \\ fs []
+QED
+
+Theorem Letrec_Lam_weak:
+  ∀l v e b. EVERY (λe. v ∉ freevars e) (MAP SND l) ∧ ¬ MEM v (MAP FST l)
+            ⇒ (Letrec l (Lam v e) ≅? Lam v (Letrec l e)) b
+Proof
+  rw [exp_eq_def, bind_def] >> IF_CASES_TAC >>
+  gvs [app_bisimilarity_eq, exp_eq_refl] >>
+  rpt $ irule_at Any IMP_closed_subst >>
+  gvs [subst_def, FDIFF_DOMSUB, MAP_subst_fdomsub] >>
+  irule_at Any Letrec_Lam >>
+  gvs [MAP_MAP_o, combinTheory.o_DEF, LAMBDA_PROD, EVERY_EL, EL_MAP] >>
+  rw [FRANGE_FLOOKUP]
+  >- (rename1 ‘EL n l’ >> qabbrev_tac ‘p = EL n l’ >>
+      PairCases_on ‘p’ >>
+      ‘∀v. v ∈ FRANGE (FDIFF f (set (MAP FST l))) ⇒ closed v’
+        by (rw [FRANGE_FLOOKUP, FLOOKUP_FDIFF] >>
+            first_x_assum irule >>
+            pop_assum $ irule_at Any) >>
+      gvs [freevars_subst, SUBSET_DEF, IN_DIFF, FDOM_FDIFF] >>
+      gen_tac >> rename1 ‘MEM x _’ >>
+      last_x_assum $ qspecl_then [‘x’] assume_tac >>
+      last_x_assum $ qspecl_then [‘x’] assume_tac >>
+      rw [] >> gvs []
+      >- (last_x_assum $ qspecl_then [‘freevars p1’] assume_tac >>
+          gvs [MEM_MAP] >> pop_assum $ qspecl_then [‘EL n l’] assume_tac >>
+          gvs [EL_MEM])
+      >- (last_x_assum $ qspecl_then [‘freevars p1’] assume_tac >>
+          gvs [MEM_MAP] >> pop_assum $ qspecl_then [‘EL n l’] assume_tac >>
+          gvs [EL_MEM]) >>
+      gvs [MEM_EL] >>
+      first_assum $ irule_at Any >>
+      rw [EL_MAP] >>
+      rename1 ‘FST p2’ >> PairCases_on ‘p2’ >> fs [])
+  >- (strip_tac >> last_x_assum irule >>
+      gvs [MEM_EL] >> first_assum $ irule_at Any >>
+      gvs [EL_MAP] >> rename1 ‘FST p’ >> PairCases_on ‘p’ >>
+      fs [])
+QED
+
+Theorem Letrec_not_in_freevars:
+  ∀l e b. EVERY (λv. v ∉ freevars e) (MAP FST l) ⇒ (Letrec l e ≅? e) b
+Proof
+  rw [exp_eq_def, bind_def] >> IF_CASES_TAC >>
+  gvs [app_bisimilarity_eq, exp_eq_refl] >>
+  rpt $ irule_at Any IMP_closed_subst >>
+  gvs [subst_def, FRANGE_FLOOKUP] >>
+  irule exp_eq_trans >>
+  irule_at Any beta_equality_Letrec >>
+  conj_asm1_tac
+  >- (rw [EVERY_EL, EL_MAP, MAP_MAP_o, combinTheory.o_DEF, LAMBDA_PROD] >>
+      rename1 ‘EL n l’ >> qabbrev_tac ‘p = EL n l’ >> PairCases_on ‘p’ >>
+      ‘∀v. v ∈ FRANGE (FDIFF f (set (MAP FST l))) ⇒ closed v’
+        by (rw [FRANGE_FLOOKUP, FLOOKUP_FDIFF] >>
+            first_x_assum irule >>
+            pop_assum $ irule_at Any) >>
+      gvs [freevars_subst, SUBSET_DEF, IN_DIFF, FDOM_FDIFF] >>
+      gen_tac >> rename1 ‘MEM x _’ >>
+      last_x_assum $ qspecl_then [‘x’] assume_tac >>
+      rw [] >> gvs []
+      >- (first_x_assum $ qspecl_then [‘freevars p1’] assume_tac >>
+          gvs [MEM_MAP] >> pop_assum $ qspecl_then [‘EL n l’] assume_tac >>
+          gvs [EL_MEM]) >>
+      gvs [MEM_EL] >>
+      first_assum $ irule_at Any >> rw [EL_MAP] >>
+      rename1 ‘FST p2’ >> PairCases_on ‘p2’ >> fs []) >>
+  dxrule_then assume_tac subst_funs_eq_subst >>
+  qspecl_then [‘f’, ‘e’, ‘set (MAP FST l)’] assume_tac $ GSYM subst_FDIFF' >>
+  gvs [EVERY_MEM] >>
+  rw [exp_eq_refl, IMP_closed_subst, FRANGE_FLOOKUP]
+QED
+
+Theorem Let_Letrec:
+  ∀s l e1 e2 b. EVERY (λe. s ∉ freevars e) (MAP SND l) ∧ ¬MEM s (MAP FST l)
+                ∧ EVERY (λv. v ∉ freevars e1) (MAP FST l)
+                ⇒ (Let s e1 (Letrec l e2) ≅? Letrec l (Let s e1 e2)) b
+Proof
+  rw [] >>
+  irule exp_eq_trans >>
+  irule_at (Pos hd) exp_eq_App_cong >>
+  irule_at (Pos hd) $ iffLR exp_eq_sym >>
+  irule_at Any Letrec_Lam_weak >> fs [] >>
+  irule_at Any exp_eq_refl >>
+  irule $ iffLR exp_eq_sym >>
+  irule exp_eq_trans >>
+  irule_at Any Letrec_App >>
+  irule exp_eq_App_cong >>
+  gvs [exp_eq_refl, Letrec_not_in_freevars]
+QED
+
+Theorem Let_Letrec2:
+  ∀s l e1 e2 b. ¬MEM s (MAP FST l)
+                ∧ EVERY (λv. v ∉ freevars e1) (MAP FST l)
+                ⇒ (Let s e1 (Letrec l e2) ≅? Letrec (MAP (λ(v, e). (v, Let s e1 e)) l)  (Let s e1 e2)) b
+Proof
+  rw [exp_eq_def, bind_def] >> IF_CASES_TAC >>
+  gvs [app_bisimilarity_eq, exp_eq_refl] >>
+  rpt $ irule_at Any IMP_closed_subst >>
+  gvs [subst_def, FRANGE_FLOOKUP] >>
+  irule exp_eq_trans >>
+  irule_at Any beta_equality >>
+  irule_at Any IMP_closed_subst >>
+  gvs [FRANGE_FLOOKUP, subst1_def, MAP_MAP_o] >>
+  rename1 ‘MEM s (MAP (FST o (λ(f', e). (f', subst (FDIFF (f \\ s) (set (MAP FST l))) e))) l)’ >>
+  ‘¬MEM s (MAP (FST o (λ(f', e). (f', subst (FDIFF (f \\ s) (set (MAP FST l))) e))) l)’
+    by (strip_tac >> first_x_assum irule >>
+        gvs [MEM_EL] >> first_assum $ irule_at Any >> gvs [EL_MAP] >>
+        rename1 ‘EL n l’ >> qabbrev_tac ‘p = EL n l’ >> PairCases_on ‘p’ >> fs []) >>
+  gvs [] >> irule exp_eq_Letrec_cong2 >>
+  irule_at Any fmap_rel_FUPDATE_LIST_same >> irule_at Any LIST_EQ >>
+  rw [EL_MAP, fmap_rel_FEMPTY, LIST_REL_EL_EQN]
+  >~[‘FST (_ (_ p)) = FST (_ (_ p))’]
+  >- (PairCases_on ‘p’ >> fs [])
+  >~[‘SND (_ (_ p)) ≅? SND (_ (_ p))’]
+  >- (PairCases_on ‘p’ >> gvs [subst_def] >>
+      gvs [EVERY_MEM] >> drule_then assume_tac $ GSYM subst_FDIFF' >>
+      ‘MAP (FST o (λ(v, e). (v, Let s e1 e))) l = MAP FST l’
+        by (irule LIST_EQ >> rw [EL_MAP] >> rename1 ‘FST (_ p)’ >> PairCases_on ‘p’ >> fs []) >>
+      gvs [FDIFF_def, fmap_domsub, INTER_COMM, Once exp_eq_sym] >>
+      irule beta_equality >>
+      gvs [IMP_closed_subst, FRANGE_FLOOKUP])
+  >- (‘MAP (FST o (λ(v, e). (v, Let s e1 e))) l = MAP FST l’
+        by (irule LIST_EQ >> rw [EL_MAP] >> rename1 ‘FST (_ p)’ >> PairCases_on ‘p’ >> fs []) >>
+      gvs [EVERY_MEM] >> drule_then assume_tac $ GSYM subst_FDIFF' >>
+      gvs [FDIFF_def, fmap_domsub, INTER_COMM, Once exp_eq_sym] >>
+      irule beta_equality >> gvs [IMP_closed_subst, FRANGE_FLOOKUP])
+QED
+
+Theorem Let_Let:
+  ∀v w e1 e2 e3 b. v ≠ w ∧ v ∉ freevars e2 ∧ w ∉ freevars e1 ⇒
+                   (Let v e1 (Let w e2 e3) ≅? Let w e2 (Let v e1 e3)) b
+Proof
+  rw []
+  \\ irule eval_IMP_exp_eq
+  \\ rw [subst_def]
+  \\ rename1 ‘subst (f \\ _ \\ _)’
+  \\ ‘∀v. v ∈ FRANGE f ⇒ closed v’ by (rw [FRANGE_FLOOKUP])
+  \\ drule $ GSYM subst_fdomsub
+  \\ last_x_assum assume_tac
+  \\ last_x_assum assume_tac
+  \\ drule $ GSYM subst_fdomsub
+  \\ rw [eval_Let, subst_def, bind1_def, IMP_closed_subst, DOMSUB_COMMUTES]
+  \\ AP_TERM_TAC
+  \\ rw [fmap_domsub, COMPL_UNION]
+  \\ irule subst1_subst1
+  \\ gvs [IMP_closed_subst]
+QED
+
+Theorem Let_Apps:
+  ∀eL v e1 e2 b. (Let v e1 (Apps e2 eL) ≅? Apps (Let v e1 e2) (MAP (Let v e1) eL)) b
+Proof
+  Induct >> rw [Apps_def, exp_eq_refl] >>
+  irule exp_eq_trans >> pop_assum $ irule_at Any >>
+  irule exp_eq_Apps_cong >> gvs [Let_App, exp_eq_l_refl]
+QED
+
+Theorem Seq_App:
+  ∀b. (App (Seq p f) e ≅? Seq p (App f e)) b
+Proof
+  irule eval_wh_IMP_exp_eq
+  \\ rw [subst_def, eval_wh_App, eval_wh_Seq]
+  \\ fs []
+QED
+
+Theorem Apps_Seq:
+  ∀eL e e' b. (Apps (Seq e e') eL ≅? Seq e (Apps e' eL)) b
+Proof
+  Induct >> rw [Apps_def, exp_eq_refl] >>
+  irule exp_eq_trans >> pop_assum $ irule_at Any >>
+  irule exp_eq_Apps_cong >> gvs [exp_eq_l_refl, Seq_App]
+QED
+
+Theorem Proj_Seq2:
+  ∀b. (Proj x i (Seq e e') ≅? Seq e (Proj x i e')) b
+Proof
+  irule eval_wh_IMP_exp_eq
+  \\ rw [subst_def, eval_wh_Proj, eval_wh_Seq]
+  \\ fs []
+QED
+
+Theorem If_Seq:
+  ∀e e' e'' e''' b. (If (Seq e e') e'' e''' ≅? Seq e (If e' e'' e''')) b
+Proof
+  rpt gen_tac
+  \\ irule eval_wh_IMP_exp_eq
+  \\ rw [subst_def, eval_wh_If, eval_wh_Seq]
+  \\ fs []
+QED
+
+Theorem Seq_comm:
+  Seq (Seq x y) z ≈ Seq (Seq y x) z
+Proof
+  irule no_err_eval_wh_IMP_exp_eq
+  \\ rw [subst_def, no_err_eval_wh_def, eval_wh_Seq]
+  \\ fs []
+  \\ Cases_on ‘eval_wh (subst f x)’
+  \\ Cases_on ‘eval_wh (subst f y)’
+  \\ fs []
+QED
+
+Theorem If_Seq2:
+  ∀e ec et ee.  If ec (Seq e et) (Seq e ee) ≈ Seq e (If ec et ee)
+Proof
+  rpt gen_tac
+  \\ irule no_err_eval_wh_IMP_exp_eq
+  \\ rw [no_err_eval_wh_def, freevars_def, subst_def, eval_wh_If, eval_wh_Seq]
+  \\ fs []
+QED
+
+Theorem IsEq_Seq:
+  ∀b e e' n i. (IsEq n i (Seq e e') ≅? Seq e (IsEq n i e')) b
+Proof
+  rpt gen_tac
+  \\ irule eval_wh_IMP_exp_eq
+  \\ rw [subst_def, eval_wh_IsEq, eval_wh_Seq]
+  \\ fs []
+QED
+
+Definition well_written_def:
+  well_written (Cons s) l = T ∧
+  well_written (Proj s i) [e] = T ∧
+  well_written (IsEq s i) [e] = T ∧
+  well_written If [e; e'; e''] = T ∧
+  well_written Seq [e; e'] = T ∧
+  well_written (AtomOp op) l = T ∧
+  well_written _ _ = F
+End
+
+Theorem not_well_written_is_fail:
+  ∀b ope l.
+    ¬ well_written ope l ⇒
+    (Prim ope l ≅? Fail) b
+Proof
+  rw []
+  \\ Cases_on ‘ope’
+  \\ fs [well_written_def]
+  \\ Cases_on ‘l’
+  >>~[‘Prim _ [] ≅? Fail’]
+  >- (fs [exp_eq_refl])
+  >- (irule eval_wh_IMP_exp_eq
+     \\ fs [subst_def, eval_wh_def, eval_wh_to_def])
+  >- (irule eval_wh_IMP_exp_eq
+     \\ fs [subst_def, eval_wh_def, eval_wh_to_def])
+  >- (irule eval_wh_IMP_exp_eq
+     \\ fs [subst_def, eval_wh_def, eval_wh_to_def])
+  \\ rename1 ‘hd::tl’
+  \\ Cases_on ‘tl’
+  \\ fs [well_written_def]
+  >>~[‘Prim _ [hd]’]
+  >- (irule eval_wh_IMP_exp_eq
+     \\ fs [subst_def, eval_wh_def, eval_wh_to_def])
+  >- (irule eval_wh_IMP_exp_eq
+     \\ fs [subst_def, eval_wh_def, eval_wh_to_def])
+  \\ rename1 ‘h0::h1::tl’
+  \\ Cases_on ‘tl’
+  \\ fs [well_written_def]
+  >~[‘Prim If (h0::h1::h2::tl)’]
+  >- (Cases_on ‘tl’
+      \\ fs [well_written_def]
+      \\ irule eval_wh_IMP_exp_eq
+      \\ fs [subst_def, eval_wh_def, eval_wh_to_def])
+  \\ irule eval_wh_IMP_exp_eq
+  \\ fs [subst_def, eval_wh_def, eval_wh_to_def]
+QED
+
+(* Part on context *)
+
+Theorem exp_eq_in_ctxt_refl:
+  ∀c e. exp_eq_in_ctxt c e e
+Proof
+  Induct
+  \\ gvs [exp_eq_in_ctxt_def, exp_eq_refl]
+QED
+
+Theorem exp_eq_in_ctxt_l_refl:
+  ∀c l. LIST_REL (exp_eq_in_ctxt c) l l
+Proof
+  gen_tac
+  \\ Induct
+  \\ fs [exp_eq_in_ctxt_refl]
+QED
+
+Theorem exp_eq_in_ctxt_sym:
+  ∀c e1 e2. exp_eq_in_ctxt c e1 e2 ⇔ exp_eq_in_ctxt c e2 e1
+Proof
+  Induct
+  \\ rw [] \\ eq_tac
+  \\ gvs [exp_eq_in_ctxt_def, exp_eq_sym]
+QED
+
+Theorem exp_eq_in_ctxt_trans:
+  ∀c e1 e2 e3. exp_eq_in_ctxt c e1 e2 ∧ exp_eq_in_ctxt c e2 e3 ⇒ exp_eq_in_ctxt c e1 e3
+Proof
+  Induct
+  \\ rw []
+  \\ gvs [exp_eq_in_ctxt_def]
+  >- (irule exp_eq_trans
+      \\ pop_assum $ irule_at Any \\ fs [])
+  \\ rw []
+  \\ last_x_assum irule
+  \\ first_x_assum $ irule_at Any
+  \\ gvs []
+QED
+
+Theorem exp_eq_IMP_exp_eq_in_ctxt:
+  ∀c e e'. e ≈ e' ⇒ exp_eq_in_ctxt c e e'
+Proof
+  Induct
+  \\ gvs [exp_eq_in_ctxt_def]
+  \\ rw []
+  \\ first_x_assum irule
+  \\ gvs [exp_eq_Letrec_cong, exp_eq_App_cong, exp_eq_Lam_cong, exp_eq_refl, exp_eq_l_refl]
+QED
+
+Theorem exp_eq_in_ctxt_Prim:
+  ∀c eL eL' ope. LIST_REL (exp_eq_in_ctxt c) eL eL' ⇒ exp_eq_in_ctxt c (Prim ope eL) (Prim ope eL')
+Proof
+  Induct
+  \\ gvs [exp_eq_in_ctxt_def, exp_eq_refl, exp_eq_Prim_cong]
+  \\ rw []
+  \\ irule exp_eq_in_ctxt_trans
+  \\ irule_at Any exp_eq_in_ctxt_trans
+  \\ last_x_assum $ irule_at Any
+  \\ irule_at (Pos last) exp_eq_IMP_exp_eq_in_ctxt
+  \\ irule_at (Pos last) exp_eq_IMP_exp_eq_in_ctxt
+  >~[‘Letrec’]
+  >- (irule_at Any Letrec_Prim
+      \\ irule_at Any $ iffLR exp_eq_sym
+      \\ irule_at Any Letrec_Prim
+      \\ gvs [LIST_REL_EL_EQN, EL_MAP, exp_eq_in_ctxt_def])
+  \\ irule_at Any Let_Prim
+  \\ irule_at Any $ iffLR exp_eq_sym
+  \\ irule_at Any Let_Prim
+  \\ gvs [LIST_REL_EL_EQN, EL_MAP, exp_eq_in_ctxt_def]
+QED
+
+Theorem Let_App_in_ctxt:
+  ∀c s e1 e2 e3. exp_eq_in_ctxt c (Let s e1 (App e2 e3)) (App (Let s e1 e2) (Let s e1 e3))
+Proof
+  rpt gen_tac
+  \\ irule exp_eq_IMP_exp_eq_in_ctxt
+  \\ gvs [Let_App]
+QED
+
+Theorem exp_eq_in_ctxt_App:
+  ∀c f1 f2 e1 e2. exp_eq_in_ctxt c f1 f2 ∧ exp_eq_in_ctxt c e1 e2
+                  ⇒ exp_eq_in_ctxt c (App f1 e1) (App f2 e2)
+Proof
+  Induct
+  \\ gvs [exp_eq_in_ctxt_def,exp_eq_App_cong]
+  \\ rw []
+  \\ irule exp_eq_in_ctxt_trans
+  \\ irule_at Any exp_eq_in_ctxt_trans
+  \\ last_x_assum $ irule_at (Pos $ el 2)
+  \\ first_x_assum $ irule_at (Pos $ el 2)
+  \\ rpt $ last_assum $ irule_at Any
+  \\ irule_at (Pos last) $ iffLR exp_eq_in_ctxt_sym
+  \\ rpt $ irule_at Any Let_App_in_ctxt
+  \\ fs [Letrec_App, exp_eq_IMP_exp_eq_in_ctxt]
+QED
+
+Theorem exp_eq_in_ctxt_Apps:
+  ∀eL eL' e e' c. LIST_REL (exp_eq_in_ctxt c) eL eL' ⇒ exp_eq_in_ctxt c e e'
+                  ⇒ exp_eq_in_ctxt c (Apps e eL) (Apps e' eL')
+Proof
+  Induct
+  >- (Cases
+      \\ fs [Apps_def])
+  \\ gen_tac
+  \\ Cases
+  \\ rw [Apps_def]
+  \\ first_x_assum irule
+  \\ fs [exp_eq_in_ctxt_App]
+QED
+
+Theorem Let_freevars:
+  ∀c v e e'. v ∉ freevars e' ⇒ exp_eq_in_ctxt c (Let v e e') e'
+Proof
+  rw []
+  \\ irule exp_eq_IMP_exp_eq_in_ctxt
+  \\ irule eval_wh_IMP_exp_eq
+  \\ rw [subst_def, eval_wh_thm, bind1_def, GSYM subst_fdomsub]
+  >- (AP_TERM_TAC
+      \\ irule subst1_ignore
+      \\ rename1 ‘subst f e2’
+      \\ qsuff_tac ‘closed (subst f e2)’
+      >- rw [closed_def]
+      \\ irule IMP_closed_subst
+      \\ rw []
+      \\ first_x_assum $ irule_at Any
+      \\ fs [FRANGE_FLOOKUP]
+      \\ pop_assum $ irule_at Any)
+  \\ gvs [IMP_closed_subst, FRANGE_FLOOKUP]
+QED
+
+Theorem Let_Let_in_ctxt:
+  ∀v w e1 e2 e3 c. v ≠ w ∧ v ∉ freevars e2 ∧ w ∉ freevars e1 ⇒
+                   exp_eq_in_ctxt c (Let v e1 (Let w e2 e3)) (Let w e2 (Let v e1 e3))
+Proof
+  rw []
+  \\ irule exp_eq_IMP_exp_eq_in_ctxt
+  \\ gvs [Let_Let]
+QED
+
+Theorem exp_eq_in_ctxt_Lam:
+  ∀c s e1 e2. exp_eq_in_ctxt (IsFree s c) e1 e2
+              ⇒ exp_eq_in_ctxt c (Lam s e1) (Lam s e2)
+Proof
+  Induct
+  \\ fs[exp_eq_in_ctxt_def] \\ rw [exp_eq_in_ctxt_def]
+  >- (rw [exp_eq_Lam_strong]
+      \\ irule exp_eq_trans
+      \\ irule_at Any beta_equality
+      \\ fs []
+      \\ irule $ iffLR exp_eq_sym
+      \\ irule exp_eq_trans
+      \\ irule_at (Pos last) beta_equality
+      \\ fs [exp_eq_sym])
+  >>~ [‘Letrec l (Lam w _)’]
+  >- (‘∃s. s ∉ {w} ∪ set (MAP FST l) ∪ BIGUNION (set (MAP (freevars o SND) l))
+             ∪ freevars e1 ∪ freevars e2’
+        by  (‘INFINITE 𝕌(:string)’ by simp [] \\ dxrule_then assume_tac $ iffLR NOT_IN_FINITE
+             \\ pop_assum $ irule_at Any \\ rw [FINITE_UNION, FINITE_BIGUNION, MEM_EL]
+             \\ gvs [EL_MAP])
+      \\ irule exp_eq_in_ctxt_trans
+      \\ irule_at (Pos hd) exp_eq_IMP_exp_eq_in_ctxt
+      \\ irule_at Any exp_eq_Letrec_cong
+      \\ irule_at Any exp_eq_l_refl
+      \\ irule_at Any exp_alpha_exp_eq
+      \\ irule_at Any exp_alpha_Alpha
+      \\ fs [] \\ first_assum $ irule_at Any
+      \\ fs []
+      \\ irule exp_eq_in_ctxt_trans
+      \\ irule_at (Pos hd) exp_eq_IMP_exp_eq_in_ctxt
+      \\ irule_at Any Letrec_Lam_weak
+      \\ fs [] \\ conj_tac
+      >- (rw [EVERY_MEM]
+          \\ rename1 ‘MEM e _’ \\ last_x_assum $ qspecl_then [‘freevars e’] assume_tac
+          \\ fs [MEM_MAP]
+          \\ rename1 ‘e = SND pair’ \\ pop_assum $ qspecl_then [‘pair’] assume_tac
+          \\ rw [])
+      \\ irule exp_eq_in_ctxt_trans
+      \\ irule_at (Pos last) exp_eq_IMP_exp_eq_in_ctxt
+      \\ irule_at Any $ iffLR exp_eq_sym
+      \\ irule_at Any exp_eq_Letrec_cong
+      \\ irule_at Any exp_alpha_exp_eq
+      \\ irule_at Any exp_alpha_Alpha
+      \\ irule_at Any exp_eq_l_refl
+      \\ first_assum $ irule_at Any \\ fs []
+      \\ irule exp_eq_in_ctxt_trans
+      \\ irule_at (Pos last) exp_eq_IMP_exp_eq_in_ctxt
+      \\ irule_at Any $ iffLR exp_eq_sym
+      \\ irule_at Any Letrec_Lam_weak
+      \\ fs []
+      \\ conj_tac
+      >- (rw [EVERY_MEM]
+          \\ rename1 ‘MEM e _’ \\ last_x_assum $ qspecl_then [‘freevars e’] assume_tac
+          \\ fs [MEM_MAP]
+          \\ rename1 ‘e = SND pair’ \\ pop_assum $ qspecl_then [‘pair’] assume_tac
+          \\ rw [])
+      \\ last_x_assum irule \\ rw []
+      \\ irule exp_eq_in_ctxt_trans
+      \\ irule_at Any exp_eq_in_ctxt_trans
+      \\ last_x_assum $ irule_at Any
+      \\ irule_at (Pos last) $ iffLR exp_eq_in_ctxt_sym
+      \\ rename1 ‘Let s e3 _’ \\ qexists_tac ‘e3’ \\ fs []
+      \\ conj_tac
+      \\ irule exp_eq_IMP_exp_eq_in_ctxt
+      \\ irule exp_eq_trans
+      \\ irule_at Any Let_Letrec
+      \\ fs []
+      \\ irule_at Any exp_eq_Letrec_cong
+      \\ irule_at Any $ iffLR exp_eq_sym
+      \\ irule_at Any exp_eq_App_cong
+      \\ irule_at Any exp_alpha_exp_eq
+      \\ irule_at Any exp_alpha_Alpha
+      \\ rw [EVERY_MEM, exp_eq_refl, exp_eq_l_refl] \\ fs [closed_def]
+      \\ rename1 ‘MEM e _’
+      \\ last_x_assum $ qspecl_then [‘freevars e’] assume_tac
+      \\ fs [MEM_MAP]
+      \\ rename1 ‘e = SND pair’ \\ pop_assum $ qspecl_then [‘pair’] assume_tac
+      \\ rw [])
+  \\ rename1 ‘Let v e3 (Lam w _)’
+  \\ ‘∃s. s ∉ {v} ∪ {w} ∪ freevars e3 ∪ freevars e1 ∪ freevars e2’
+    by (‘INFINITE 𝕌(:string)’ by simp []
+        \\ gvs [NOT_IN_FINITE])
+  \\ irule exp_eq_in_ctxt_trans
+  \\ irule_at (Pos hd) exp_eq_IMP_exp_eq_in_ctxt
+  \\ irule_at Any exp_eq_App_cong \\ irule_at Any exp_eq_Lam_cong
+  \\ irule_at Any exp_alpha_exp_eq
+  \\ irule_at Any exp_alpha_Alpha
+  \\ fs [] \\ first_assum $ irule_at Any
+  \\ irule_at Any exp_eq_refl \\ fs []
+  \\ irule exp_eq_in_ctxt_trans
+  \\ irule_at (Pos hd) exp_eq_IMP_exp_eq_in_ctxt
+  \\ irule_at Any Let_Lam_weak \\ fs []
+  \\ irule exp_eq_in_ctxt_trans
+  \\ irule_at (Pos last) exp_eq_IMP_exp_eq_in_ctxt
+  \\ irule_at Any $ iffLR exp_eq_sym
+  \\ irule_at Any exp_eq_App_cong \\ irule_at Any exp_eq_Lam_cong
+  \\ irule_at Any exp_alpha_exp_eq
+  \\ irule_at Any exp_alpha_Alpha
+  \\ first_assum $ irule_at Any
+  \\ irule_at Any exp_eq_refl \\ fs []
+  \\ irule exp_eq_in_ctxt_trans
+  \\ irule_at (Pos last) exp_eq_IMP_exp_eq_in_ctxt
+  \\ irule_at Any $ iffLR exp_eq_sym
+  \\ irule_at Any Let_Lam_weak \\ fs []
+  \\ last_x_assum $ irule_at Any
+  \\ rw []
+  \\ irule exp_eq_in_ctxt_trans \\ irule_at Any exp_eq_in_ctxt_trans
+  \\ last_x_assum $ irule_at Any
+  \\ rpt $ irule_at Any exp_eq_IMP_exp_eq_in_ctxt
+  \\ irule_at (Pos $ el 2) $ iffLR exp_eq_sym
+  \\ irule_at (Pos $ el 2) exp_eq_trans \\ irule_at (Pos $ el 3) exp_eq_trans
+  \\ irule_at (Pos $ el 2) Let_Let \\ irule_at (Pos $ el 6) Let_Let
+  \\ rpt $ irule_at Any exp_eq_App_cong
+  \\ rpt $ irule_at Any exp_eq_refl
+  \\ rpt $ irule_at Any exp_eq_Lam_cong
+  \\ rpt $ irule_at Any exp_eq_App_cong
+  \\ rpt $ irule_at Any exp_eq_refl
+  \\ fs [closed_def] \\ conj_tac
+  \\ irule exp_alpha_exp_eq
+  \\ irule exp_alpha_Alpha
+  \\ fs []
+QED
+
+Theorem exp_eq_in_ctxt_Lams:
+  ∀vl c e e'. exp_eq_in_ctxt (FOLDL (λc n. IsFree n c) c vl) e e' ⇒
+              exp_eq_in_ctxt c (Lams vl e) (Lams vl e')
+Proof
+  Induct
+  \\ rw [Lams_def]
+  \\ irule exp_eq_in_ctxt_Lam
+  \\ last_x_assum $ irule_at Any
+  \\ fs []
+QED
+
+Theorem exp_eq_in_IsFree_Bind:
+  ∀e1 e2 e3 c v. exp_eq_in_ctxt (IsFree v c) e1 e2 ⇒ exp_eq_in_ctxt (Bind v e3 c) e1 e2
+Proof
+  rpt strip_tac >>
+  gvs [exp_eq_in_ctxt_def, exp_eq_in_ctxt_App, exp_eq_in_ctxt_Lam, exp_eq_in_ctxt_refl]
+QED
+
+Theorem Apps_Seq_in_ctxt:
+  ∀e e2 eL c. exp_eq_in_ctxt c (Apps (Seq e e2) eL) (Seq e (Apps e2 eL))
+Proof
+  rw [exp_eq_IMP_exp_eq_in_ctxt, Apps_Seq]
+QED
+
+Theorem Let_Apps_in_ctxt:
+  ∀v e1 e2 eL c. exp_eq_in_ctxt c (Let v e1 (Apps e2 eL)) (Apps (Let v e1 e2) (MAP (Let v e1) eL))
+Proof
+  rw [Let_Apps, exp_eq_IMP_exp_eq_in_ctxt]
+QED
+
+Theorem Letrec_Apps:
+  ∀l bL b e. (Letrec bL (Apps e l) ≅? Apps (Letrec bL e) (MAP (Letrec bL) l)) b
+Proof
+  Induct >> gvs [exp_eq_refl, Apps_def] >>
+  rpt gen_tac >>
+  irule exp_eq_trans >> pop_assum $ irule_at Any >>
+  irule exp_eq_Apps_cong >>
+  fs [exp_eq_l_refl, Letrec_App]
+QED
+
+Theorem Letrec_Apps_in_ctxt:
+  ∀l b e c. exp_eq_in_ctxt c (Letrec b (Apps e l)) (Apps (Letrec b e) (MAP (Letrec b) l))
+Proof
+  gvs [exp_eq_IMP_exp_eq_in_ctxt, Letrec_Apps]
+QED
+
+Definition unfold_ctxt_def:
+  unfold_ctxt Nil e = e ∧
+  unfold_ctxt (IsFree v c) e = Lam v (unfold_ctxt c e) ∧
+  unfold_ctxt (Bind v e c) e2 = Let v e (unfold_ctxt c e2) ∧
+  unfold_ctxt (RecBind bL c) e = Letrec bL (unfold_ctxt c e)
+End
+
+Definition concat_ctxt_def:
+  concat_ctxt Nil c = c ∧
+  concat_ctxt (IsFree v c1) c2 = concat_ctxt c1 (IsFree v c2) ∧
+  concat_ctxt (Bind v e c1) c2 = concat_ctxt c1 (Bind v e c2) ∧
+  concat_ctxt (RecBind bL c1) c2 = concat_ctxt c1 (RecBind bL c2)
+End
+
+Definition not_bound_in_ctxt_def:
+  not_bound_in_ctxt Nil v = T ∧
+  not_bound_in_ctxt (IsFree v1 c) v2 = (v1 ≠ v2 ∧ not_bound_in_ctxt c v2) ∧
+  not_bound_in_ctxt (Bind v1 e c) v2 = (v1 ≠ v2 ∧ not_bound_in_ctxt c v2) ∧
+  not_bound_in_ctxt (RecBind bL c) v = (not_bound_in_ctxt c v ∧ ¬MEM v (MAP FST bL))
+End
+
+Theorem Let_stay:
+  ∀v e b. v ∉ freevars e ⇒ (Let v e (Var v) ≅? Let v e e) b
+Proof
+  rw [] >> irule exp_eq_trans >>
+  irule_at Any Let_Var >>
+  irule eval_IMP_exp_eq >>
+  rw [eval_thm, subst_def, GSYM subst_fdomsub, bind1_def, subst1_ignore, closed_def, IMP_closed_subst,
+      FRANGE_FLOOKUP]
+QED
+
+Theorem exp_eq_in_ctxt_unfold:
+  ∀c2 w e' c1. not_bound_in_ctxt c2 w ∧ (∀v. v ∈ freevars e' ⇒ not_bound_in_ctxt c2 v) ∧ w ∉ freevars e'
+              ⇒ exp_eq_in_ctxt (Bind w e' c1) (unfold_ctxt c2 (Var w)) (unfold_ctxt c2 e')
+Proof
+  Induct >> rw [not_bound_in_ctxt_def, exp_eq_in_ctxt_def, unfold_ctxt_def]
+  >- gvs [exp_eq_in_ctxt_def, exp_eq_IMP_exp_eq_in_ctxt, Let_stay] >>
+  irule exp_eq_in_ctxt_trans >> irule_at Any exp_eq_in_ctxt_trans >>
+  irule_at (Pos hd) exp_eq_IMP_exp_eq_in_ctxt >> irule_at (Pos last) exp_eq_IMP_exp_eq_in_ctxt >>
+  irule_at (Pos hd) $ iffLR exp_eq_sym >~[‘Letrec’]
+  >- (rpt $ irule_at Any Let_Letrec2 >>
+      gvs [GSYM exp_eq_in_ctxt_def, EVERY_MEM] >>
+      rw [] >> strip_tac >> first_x_assum $ dxrule_then assume_tac >>
+      gvs [])
+  >- (rpt $ irule_at Any Let_Lam_weak >>
+      irule_at Any exp_eq_in_ctxt_Lam >>
+      gvs [GSYM exp_eq_in_ctxt_def] >>
+      strip_tac >> first_x_assum $ dxrule_then assume_tac >> fs [])
+  >- cheat
+QED
+
+(** end ctxt **)
 
 Definition Projs_def:
   Projs [] e = e ∧
@@ -79,6 +979,19 @@ Proof
   \\ conj_tac THEN1 fs []
   \\ irule exp_eq_Projs_cong
   \\ fs [Let_Prim_alt]
+QED
+
+Theorem Letrec_Projs:
+  ∀ps x bL b. (Letrec bL (Projs ps x) ≅? Projs ps (Letrec bL x)) b
+Proof
+  Induct \\ fs [Projs_def,exp_eq_refl,FORALL_PROD] \\ rw []
+  \\ irule exp_eq_trans
+  \\ qexists_tac ‘Projs ps (Letrec bL (Proj p_1 p_2 x))’
+  \\ conj_tac THEN1 fs []
+  \\ irule exp_eq_Projs_cong
+  \\ irule exp_eq_trans
+  \\ irule_at Any Letrec_Prim
+  \\ gvs [exp_eq_refl]
 QED
 
 Theorem Projs_subst:
@@ -760,8 +1673,41 @@ QED
 val _ = set_fixity "fdemands" (Infixl 480);
 
 Definition fdemands_def:
-  f fdemands ((ps, i), len, c) = (i < len ∧ ∀l. LENGTH l = len ⇒ (Apps f l) needs ((ps, EL i l), c))
+  f fdemands ((ps, i), len, Nil) = (i < len ∧ (∀l. LENGTH l = len ⇒ Apps f l needs ((ps, EL i l), Nil))) ∧
+  f fdemands (p, len, Bind v e c) = (Let v e f) fdemands (p, len, c) ∧
+  f fdemands (p, len, RecBind b c) = (Letrec b f) fdemands (p, len, c) ∧
+  f fdemands (p, len, IsFree v c) = ∀e. (Let v e f) fdemands (p, len, c)
 End
+
+Theorem fdemands_alt:
+  ∀(c : ctxt) f ps i len. f fdemands ((ps, i), len, c) ⇒ i < len ∧ ∀l. LENGTH l = len ⇒ (Apps f l) needs ((ps, EL i l), c)
+Proof
+  Induct >> gvs [fdemands_def] >> rpt gen_tac >> strip_tac
+  >~[‘IsFree’]
+  >- (rw [needs_def, exp_eq_in_ctxt_def]
+      >- (pop_assum $ qspecl_then [‘Fail’] assume_tac >> last_x_assum $ dxrule_then assume_tac >> fs []) >>
+      gvs [needs_def] >>
+      irule exp_eq_in_ctxt_trans >> irule_at Any Let_Apps_in_ctxt >>
+      rename1 ‘Let s e3 _’ >> first_x_assum $ qspecl_then [‘e3’] assume_tac >>
+      irule exp_eq_in_ctxt_trans >> last_x_assum $ dxrule_then assume_tac >>
+      fs [] >> first_x_assum $ irule_at Any >> fs [EL_MAP] >>
+      irule exp_eq_IMP_exp_eq_in_ctxt >> irule $ iffLR exp_eq_sym >>
+      irule exp_eq_trans >> irule_at Any Let_Seq >>
+      gvs [Let_Projs, exp_eq_Prim_cong, Let_Apps])
+  >~[‘Bind’]
+  >- (last_x_assum $ dxrule_then assume_tac >> fs [needs_def, exp_eq_in_ctxt_def] >> rw [] >>
+      irule exp_eq_in_ctxt_trans >> irule_at Any Let_Apps_in_ctxt >>
+      irule_at Any exp_eq_in_ctxt_trans >> first_x_assum $ irule_at Any >> fs [EL_MAP] >>
+      irule exp_eq_IMP_exp_eq_in_ctxt >> irule $ iffLR exp_eq_sym >>
+      irule exp_eq_trans >> irule_at Any Let_Seq >>
+      gvs [Let_Projs, exp_eq_Prim_cong, Let_Apps]) >>
+  last_x_assum $ dxrule_then assume_tac >> fs [needs_def, exp_eq_in_ctxt_def] >> rw [] >>
+  irule exp_eq_in_ctxt_trans >> irule_at Any Letrec_Apps_in_ctxt >>
+  irule_at Any exp_eq_in_ctxt_trans >> first_x_assum $ irule_at Any >> fs [EL_MAP] >>
+  irule exp_eq_IMP_exp_eq_in_ctxt >> irule $ iffLR exp_eq_sym >>
+  irule exp_eq_trans >> irule_at Any Letrec_Prim >>
+  gvs [Letrec_Projs, exp_eq_Prim_cong, Letrec_Apps]
+QED
 
 val _ = set_fixity "fdemands_depth" (Infixl 480);
 
@@ -1053,15 +1999,38 @@ Proof
   \\ fs [EL_MAP]
 QED
 
-Theorem fdemands_Seq:
-  ∀fd e1 e2. e2 fdemands fd ⇒ (Seq e1 e2) fdemands fd
+Theorem fdemands_exp_eq:
+  ∀c p f f' len. exp_eq_in_ctxt c f f' ∧ f fdemands (p, len, c) ⇒ f' fdemands (p, len, c)
 Proof
-  PairCases >> rw [fdemands_def] >>
-  irule needs_exp_eq >>
-  irule_at Any needs_Seq2 >>
-  last_x_assum $ irule_at Any >>
-  irule_at Any exp_eq_IMP_exp_eq_in_ctxt >> once_rewrite_tac [exp_eq_sym] >>
-  irule_at Any Apps_Seq >> fs []
+  Induct
+  >- (PairCases >> rw [fdemands_def] >>
+      irule needs_exp_eq >> pop_assum $ irule_at Any >>
+      gvs [exp_eq_in_ctxt_Apps, exp_eq_in_ctxt_l_refl])
+  >~[‘IsFree’]
+  >- (rw [fdemands_def] >> last_x_assum irule >>
+      pop_assum $ irule_at Any >> irule_at Any exp_eq_in_ctxt_App >>
+      irule_at Any exp_eq_in_ctxt_refl >> irule_at Any exp_eq_in_ctxt_Lam >>
+      fs []) >>
+  rw [fdemands_def, exp_eq_in_ctxt_def] >> last_x_assum irule >>
+  rpt $ pop_assum $ irule_at Any
+QED
+
+Theorem fdemands_Seq:
+  ∀c p len e1 e2. e2 fdemands (p, len, c) ⇒ (Seq e1 e2) fdemands (p, len, c)
+Proof
+  Induct
+  >- (PairCases >> rw [fdemands_def] >>
+      irule needs_exp_eq >> irule_at Any needs_Seq2 >> pop_assum $ irule_at Any >>
+      gvs [exp_eq_in_ctxt_def, Once exp_eq_sym] >> irule_at Any Apps_Seq) >>
+  rw [fdemands_def] >>
+  irule fdemands_exp_eq >> last_x_assum $ irule_at Any >>
+  pop_assum $ irule_at Any >>
+  once_rewrite_tac [exp_eq_in_ctxt_sym]
+  >~[‘Letrec’]
+  >- (irule_at Any exp_eq_IMP_exp_eq_in_ctxt >>
+      irule_at Any exp_eq_trans >> irule_at Any Letrec_Prim >>
+      gvs [] >> rpt $ irule_at Any exp_eq_refl) >>
+  irule_at Any exp_eq_IMP_exp_eq_in_ctxt >> irule_at Any Let_Seq
 QED
 
 (*Theorem fdemands_every_thing:
@@ -1510,7 +2479,7 @@ Definition dest_fd_SND_def:
   dest_fd_SND NONE = {} ∧
   dest_fd_SND (SOME (bL, s)) = s
 End
-        
+
 Inductive find: (* i i i o o o *)
 [find_Drop_fd:]
   (∀e e' c fds ds fd.
@@ -1625,12 +2594,12 @@ Inductive find: (* i i i o o o *)
      find e (FOLDL (λc n. IsFree n c) c vl) fdc ds e' fd
      ∧ EVERY (λv. ∀argDs. (v, argDs) ∉ fdc) vl
      ⇒ find (Lams vl e) c fdc {} (Lams vl e') NONE ) ∧
-[find_Lams_fd:] 
-  (∀e e' c ds vl fdc fd bL1 bL2.
-     find e (FOLDL (λc n. IsFree n c) c vl) fdc ds e' (SOME (bL1, fd))
+[find_Lams_fd:]
+  (∀e e' c ds vl fdc bL.
+     find e (FOLDL (λc n. IsFree n c) c vl) fdc ds e' NONE
      ∧ EVERY (λv. ∀argDs. (v, argDs) ∉ fdc) vl
-     ∧ LIST_REL (λv b. if b then ∃ps. (ps, v) ∈ ds else T) vl bL2
-     ⇒ find (Lams vl e) c fdc {} (Lams vl e') (SOME (bL2 ++ bL1, {}))) ∧
+     ∧ LIST_REL (λv b. if b then ∃ps. (ps, v) ∈ ds else T) vl bL
+     ⇒ find (Lams vl e) c fdc {} (Lams vl e') (SOME (bL, {}))) ∧
 [find_Eq:]
   (∀e e' c fdc. exp_eq_in_ctxt c e e' ⇒ find e c fdc {} e' NONE) ∧
 [find_Letrec:]
@@ -1647,16 +2616,8 @@ fun apply_to_first_n 0 tac = ALL_TAC
 Theorem fdemands_IsFree:
   ∀d c v e len. v ∉ freevars e ∧ e fdemands (d, len, c) ⇒ e fdemands (d, len, IsFree v c)
 Proof
-  PairCases >> rw [fdemands_def, needs_def, exp_eq_in_ctxt_def] >>
-  irule exp_eq_in_ctxt_trans >> irule_at Any Let_Apps_in_ctxt >>
-  irule_at (Pos hd) exp_eq_in_ctxt_trans >> irule_at Any exp_eq_in_ctxt_Apps >>
-  irule_at Any exp_eq_in_ctxt_l_refl >> irule_at Any exp_eq_IMP_exp_eq_in_ctxt >>
-  irule_at Any exp_eq_in_ctxt_trans >> first_x_assum $ irule_at Any >>
-  gvs [Once exp_eq_in_ctxt_sym] >> irule_at Any exp_eq_IMP_exp_eq_in_ctxt >>
-  irule_at (Pos hd) exp_eq_trans >> irule_at Any Let_Seq >>
-  irule_at Any exp_eq_Prim_cong >>  gvs [EL_MAP, Let_Projs] >>
-  irule_at (Pos hd) exp_eq_trans >> irule_at Any Let_Apps >>
-  irule_at Any exp_eq_Apps_cong >> gvs [exp_eq_l_refl] >>
+  rw [fdemands_def] >> irule fdemands_exp_eq >> first_x_assum $ irule_at Any >>
+  irule exp_eq_IMP_exp_eq_in_ctxt >>
   irule eval_IMP_exp_eq >> dxrule $ GSYM subst_fdomsub >>
   rw [subst_def, eval_thm, IMP_closed_subst, FRANGE_FLOOKUP, bind1_def]
 QED
@@ -1664,40 +2625,33 @@ QED
 Theorem fdemands_Bind:
   ∀d c v e e2 len. v ∉ freevars e ∧ e fdemands (d, len, c) ⇒ e fdemands (d, len, Bind v e2 c)
 Proof
-  PairCases >> rw [] >>
-  dxrule_then (dxrule_then assume_tac) fdemands_IsFree >>
-  gvs [fdemands_def, needs_in_IsFree_Bind]
+  rw [fdemands_def] >> irule fdemands_exp_eq >> first_x_assum $ irule_at Any >>
+  irule exp_eq_IMP_exp_eq_in_ctxt >>
+  irule eval_IMP_exp_eq >> dxrule $ GSYM subst_fdomsub >>
+  rw [subst_def, eval_thm, IMP_closed_subst, FRANGE_FLOOKUP, bind1_def]
 QED
 
-(*Theorem fdemands_Letrec:
-  ∀d c b e len. e fdemands (d, len, RecBind b c) ⇒ Letrec b e fdemands (d, len, c)
-Proof
-  PairCases >> rw [fdemands_def, needs_def, exp_eq_in_ctxt_def] >>
-  rename1 ‘Apps (Letrec b e) l’ >>
-  qspecl_then [‘BIGUNION (set (MAP freevars l))’, ‘b’, ‘e’, ‘F’] assume_tac Letrec_rename1 >>
-  gvs [] >> irule needs_exp_eq >>
-  dxrule_then assume_tac exp_eq_IMP_exp_eq_in_ctxt >>
-  irule_at Any exp_eq_in_ctxt_Apps >> irule_at Any exp_eq_in_ctxt_l_refl >>
-  once_rewrite_tac [exp_eq_in_ctxt_sym] >>
-  first_assum $ irule_at Any >>
-  last_x_assum $ qspecl_then >>
-              gvs [needs_def, exp_eq_in_ctxt_def] >>
-  cheat
-QED*)
-
 Theorem fdemands_App:
-  ∀e e2 ps i len c. e fdemands ((ps, SUC i), SUC len, c) ⇒ App e e2 fdemands  ((ps, i), len, c)
+  ∀c e e2 ps i len. e fdemands ((ps, SUC i), SUC len, c) ⇒ App e e2 fdemands  ((ps, i), len, c)
 Proof
-  rw [fdemands_def, GSYM Apps_def] >>
-  rename1 ‘e2::l’ >> pop_assum $ qspecl_then [‘e2::l’] assume_tac >>
-  gvs []
+  Induct
+  >- (rw [fdemands_def, GSYM Apps_def] >>
+      rename1 ‘e2::l’ >> pop_assum $ qspecl_then [‘e2::l’] assume_tac >>
+      gvs []) >>
+  rw [fdemands_def] >> irule fdemands_exp_eq >>
+  rpt $ last_x_assum $ irule_at Any >>
+  irule_at Any $ iffLR exp_eq_in_ctxt_sym
+  >~[‘Letrec’] >- (irule_at Any exp_eq_IMP_exp_eq_in_ctxt >> irule_at Any Letrec_App) >>
+  irule_at Any Let_App_in_ctxt
 QED
 
 Theorem fdemands_App2:
   ∀d e e2 eL len c. e fdemands (([], 0), SUC len, c) ∧ e2 demands (d, c) ∧ LENGTH eL = len
             ⇒ Apps (App e e2) eL demands (d, c)
 Proof
-  PairCases >> rw [fdemands_def, GSYM Apps_def, GSYM needs_Var_is_demands] >>
+  PairCases >> rw [] >>
+  dxrule_then assume_tac fdemands_alt >>
+  gvs [fdemands_def, GSYM Apps_def, GSYM needs_Var_is_demands] >>
   rename1 ‘e2::eL’ >> last_x_assum $ qspecl_then [‘e2::eL’] assume_tac >>
   irule needs_trans >>
   pop_assum $ irule_at Any >>
@@ -1763,6 +2717,17 @@ Proof
   irule exp_eq_Apps_cong >> gvs [exp_eq_l_refl, Letrec_App]
 QED
 
+Theorem fdemands_RecBind:
+  ∀c p l e b. e fdemands (p, l, c)
+              ∧ EVERY (λv. v ∉ freevars e) (MAP FST b)
+              ⇒ e fdemands (p, l, RecBind b c)
+Proof
+  rw [fdemands_def] >> irule fdemands_exp_eq >>
+  last_x_assum $ irule_at Any >>
+  irule exp_eq_IMP_exp_eq_in_ctxt >> irule $ iffLR exp_eq_sym >>
+  gvs [Letrec_not_in_freevars]
+QED
+
 Theorem fdemands_set_RecBind:
   ∀fdc c b.
     (∀n l i. (n, l) ∈ fdc ∧ i < LENGTH l ∧ EL i l ⇒ Var n fdemands (([], i), LENGTH l, c))
@@ -1770,48 +2735,138 @@ Theorem fdemands_set_RecBind:
     ⇒ (∀n l i. (n, l) ∈ fdc ∧ i < LENGTH l ∧ EL i l
                ⇒ Var n fdemands (([], i), LENGTH l, RecBind b c))
 Proof
-  rw [] >> last_x_assum $ drule_then $ drule_then $ drule_then assume_tac >>
-  gvs [fdemands_def, needs_def, Projs_def, exp_eq_in_ctxt_def] >> rw [] >>
-  irule exp_eq_in_ctxt_trans >> irule_at (Pos hd) exp_eq_IMP_exp_eq_in_ctxt >>
-  irule_at Any Letrec_Apps >>
-  irule exp_eq_in_ctxt_trans >> irule_at (Pos last) exp_eq_IMP_exp_eq_in_ctxt >>
-  once_rewrite_tac [exp_eq_sym] >> irule_at Any Letrec_Prim >>
-  irule exp_eq_in_ctxt_trans >> irule_at Any exp_eq_in_ctxt_Apps >>
-  irule_at Any exp_eq_in_ctxt_l_refl >>
-  irule_at (Pos hd) exp_eq_IMP_exp_eq_in_ctxt >>
-  irule_at Any Letrec_not_in_freevars >>
-  conj_asm1_tac
-  >- (gvs [EVERY_EL] >> rpt strip_tac >> gvs []) >>
-  fs [] >> ‘∀(f: exp -> exp) i l. i < LENGTH l ⇒ f (EL i l) = EL i (MAP f l)’ by fs [EL_MAP] >>
-  gvs [] >> pop_assum kall_tac >>
-  irule exp_eq_in_ctxt_trans >> last_x_assum $ irule_at Any >> fs [] >>
-  irule exp_eq_in_ctxt_Prim >> fs [exp_eq_in_ctxt_refl] >>
-  irule exp_eq_IMP_exp_eq_in_ctxt >>
-  once_rewrite_tac [exp_eq_sym] >> irule exp_eq_trans >>
-  irule_at Any Letrec_Apps >> irule exp_eq_Apps_cong >>
-  fs [Letrec_not_in_freevars, exp_eq_l_refl]
+  rw [] >> irule fdemands_RecBind >>
+  gvs [EVERY_EL, EL_MAP] >> rw [] >> strip_tac >>
+  first_x_assum $ dxrule_then assume_tac >> gvs []
 QED
 
-Theorem fdemands_Let:
-  ∀v e e' c d len. e fdemands (d, len, Bind v e' c) ⇒ Let v e' e fdemands (d, len, c)
+Theorem Let_Let_nothing:
+  ∀e s v b. v ≠ s ∧ s ∉ freevars e ⇒ (Let s (Var v) (Let v (Var s) e) ≅? e) b
 Proof
-  cheat
-QED
-
-Theorem fdemands_exp_eq:
-  ∀d len c e e'. exp_eq_in_ctxt c e e' ∧ e fdemands (d, len, c) ⇒ e' fdemands (d, len, c)
-Proof
-  cheat
+  Induct using freevars_ind >> rpt strip_tac
+  >~[‘Let s _ (Let v _ (Var n))’]
+  >- (irule eval_IMP_exp_eq >>
+      rw [Once eval_thm, subst_def] >>
+      Cases_on ‘FLOOKUP f v’
+      >~[‘FLOOKUP f v = NONE’] >- gvs [FLOOKUP_DEF] >>
+      first_assum $ drule_then assume_tac >>
+      Cases_on ‘n = v’ >>
+      gvs [eval_thm, bind1_def, subst1_def, DOMSUB_FLOOKUP, DOMSUB_FLOOKUP_NEQ, FLOOKUP_UPDATE] >>
+      Cases_on ‘FLOOKUP f n’ >> gvs [FLOOKUP_DEF])
+  >~[‘Prim’]
+  >- (irule exp_eq_trans >>
+      irule_at Any exp_eq_App_cong >> irule_at Any exp_eq_Lam_cong >>
+      irule_at Any Let_Prim >> irule_at Any exp_eq_refl >>
+      irule_at Any exp_eq_trans >> irule_at Any Let_Prim >>
+      irule exp_eq_Prim_cong >> rw [LIST_REL_EL_EQN, EL_MAP] >>
+      last_x_assum irule >> gvs [EL_MEM] >>
+      rename1 ‘EL n es’ >> last_x_assum $ qspecl_then [‘freevars (EL n es)’] assume_tac >> fs [] >>
+      strip_tac >> first_x_assum irule >> gvs [MEM_EL] >>
+      first_assum $ irule_at Any >> fs [EL_MAP])
+  >~[‘Let s _ (Let v _ (App _ _))’]
+  >- (irule exp_eq_trans >>
+      irule_at (Pos hd) exp_eq_App_cong >> irule_at Any exp_eq_Lam_cong >>
+      irule_at Any Let_App >> irule_at Any exp_eq_refl >>
+      irule exp_eq_trans >> irule_at Any Let_App >>
+      fs [exp_eq_App_cong])
+  >~[‘Let s _ (Let v _ (Lam n e))’]
+  >- (Cases_on ‘v = n’ >> rw []
+      >~[‘Let _ _ (Let v _ (Lam v e))’]
+      >- (irule exp_eq_trans >>
+          irule_at Any exp_eq_App_cong >> irule_at (Pos hd) exp_eq_Lam_cong >>
+          irule_at (Pos $ el 2) exp_eq_refl >>
+          qexists_tac ‘Lam v e’ >> conj_tac >>
+          irule eval_IMP_exp_eq >> rw [Ntimes subst_def 2] >>
+          rename1 ‘subst (f \\ _)’ >> qspecl_then [‘f’, ‘Lam v e’] assume_tac $ GSYM subst_fdomsub >>
+          gvs [eval_thm, bind1_def, subst1_ignore, IMP_closed_subst, FRANGE_FLOOKUP]) >>
+      ‘∃s2. s2 ∉ freevars (Lam n e) ∪ {n} ∪ {v} ∪ {s} ’
+        by (‘INFINITE 𝕌(:string)’ by simp [] >> gvs [NOT_IN_FINITE]) >>
+      irule exp_eq_trans >> irule_at Any exp_eq_App_cong >>
+      irule_at (Pos hd) exp_alpha_exp_eq >> irule_at Any exp_alpha_Alpha >>
+      qexists_tac ‘s2’ >> once_rewrite_tac [perm_exp_def] >> irule_at Any exp_eq_refl >>
+      irule_at Any exp_eq_trans >> irule_at Any exp_eq_App_cong >>
+      irule_at (Pos hd) exp_eq_Lam_cong >> irule_at (Pos hd) exp_eq_App_cong >>
+      once_rewrite_tac [perm_exp_def] >>
+      irule_at (Pos hd) exp_eq_Lam_cong >> irule_at (Pos hd) $ iffLR exp_eq_sym >>
+      irule_at (Pos hd) exp_alpha_exp_eq >> irule_at (Pos hd) exp_alpha_perm_irrel >>
+      rpt $ irule_at Any exp_eq_refl >> gvs [perm_exp_def, perm1_def] >>
+      irule exp_eq_trans >>
+      irule_at Any exp_eq_App_cong >> irule_at (Pos hd) exp_eq_Lam_cong >>
+      irule_at Any Let_Lam_weak >> irule_at Any exp_eq_refl >>
+      irule_at Any exp_eq_trans >> irule_at Any Let_Lam_weak >>
+      irule_at Any exp_eq_Lam_cong >> last_x_assum $ irule_at Any >>
+      gvs [])
+  >~[‘Let s _ (Let w _ (Letrec lcs _))’]
+  >- (Cases_on ‘MEM w (MAP FST lcs)’
+      >~[‘¬MEM w (MAP FST lcs)’]
+      >- (‘∃s2. s2 ∉ freevars e ∪ BIGUNION (set (MAP freevars (MAP SND lcs)))
+                   ∪ {w} ∪ set (MAP FST lcs) ∪ {s}’
+            by (‘INFINITE 𝕌(:string)’ by simp [] >>
+                dxrule_then irule $ iffLR NOT_IN_FINITE >>
+                gvs [NOT_IN_FINITE, FINITE_BIGUNION, MEM_MAP] >>
+                rw [] >> fs [freevars_FINITE]) >>
+          irule exp_eq_trans >> irule_at Any exp_eq_App_cong >>
+          irule_at (Pos hd) exp_alpha_exp_eq >> irule_at Any exp_alpha_Alpha >>
+          qexists_tac ‘s2’ >> once_rewrite_tac [perm_exp_def] >> irule_at Any exp_eq_refl >>
+          irule_at Any exp_eq_trans >> irule_at Any exp_eq_App_cong >>
+          irule_at (Pos hd) exp_eq_Lam_cong >> irule_at (Pos hd) exp_eq_App_cong >>
+          once_rewrite_tac [perm_exp_def] >>
+          irule_at (Pos hd) exp_eq_Lam_cong >> irule_at (Pos hd) $ iffLR exp_eq_sym >>
+          irule_at (Pos hd) exp_alpha_exp_eq >> irule_at (Pos hd) exp_alpha_perm_irrel >>
+          rpt $ irule_at Any exp_eq_refl >> first_x_assum $ irule_at (Pos hd) >>
+          gvs [perm_exp_def, perm1_def, MAP_MAP_o, combinTheory.o_DEF, LAMBDA_PROD] >>
+          irule exp_eq_trans >>
+          irule_at Any exp_eq_App_cong >> irule_at Any exp_eq_Lam_cong >>
+          irule_at Any Let_Letrec2 >> irule_at Any exp_eq_refl >>
+          irule_at (Pos last) exp_eq_trans >> irule_at (Pos hd) Let_Letrec2 >>
+          irule_at Any exp_eq_Letrec_cong2 >>
+          first_x_assum $ irule_at (Pos $ el 2) >>
+          irule_at Any fmap_rel_FUPDATE_LIST_same >> irule_at Any LIST_EQ >>
+          irule_at Any $ iffRL LIST_REL_EL_EQN >>
+          gvs [EL_MAP, EVERY_EL, MEM_EL] >>
+          rw [] >> rename1 ‘n < LENGTH lcs’ >> qabbrev_tac ‘p = EL n lcs’ >> PairCases_on ‘p’ >> gvs [EL_MAP]
+          >- (last_x_assum irule >> first_assum $ irule_at Any >> gvs [] >>
+              first_x_assum $ qspecl_then [‘freevars p1’] assume_tac >> fs [] >>
+              pop_assum $ qspecl_then [‘n’] assume_tac >> gvs [EL_MAP])
+          >- (strip_tac >> first_x_assum $ qspecl_then [‘n’] assume_tac >> gvs [EL_MAP])
+          >- (strip_tac >> last_x_assum $ qspecl_then [‘n’] assume_tac >> gvs [EL_MAP])
+          >- (strip_tac >> first_x_assum $ qspecl_then [‘n’] assume_tac >> gvs [EL_MAP]))
+      >- (irule exp_eq_trans >> irule_at Any exp_eq_App_cong >> irule_at (Pos hd) exp_eq_Lam_cong >>
+          irule_at (Pos $ el 2) exp_eq_refl >>
+          qexists_tac ‘Letrec lcs e’ >> conj_tac >>
+          irule eval_IMP_exp_eq >> rw [Ntimes subst_def 2] >>
+          rename1 ‘subst (f \\ _ )’ >> qspecl_then [‘f’, ‘Letrec lcs e’] assume_tac $ GSYM subst_fdomsub >>
+          gvs [eval_thm, bind1_def, subst1_ignore, IMP_closed_subst, FRANGE_FLOOKUP]))
 QED
 
 Theorem demands_Apps2:
-  ∀v e e2 eL v d c.
+  ∀d v e e2 eL v c.
     (∀eL'. LENGTH eL' = LENGTH eL ⇒ Apps e2 eL' demands (d, Bind v e c)) ∧ v ≠ SND d
     ⇒ Apps (Let v e e2) eL demands (d, c)
 Proof
-  cheat
+  PairCases >> rw [GSYM needs_Var_is_demands, needs_def, exp_eq_in_ctxt_def] >>
+  ‘∃s. s ∉ freevars (Let v e e2) ∪ {d1} ∪ BIGUNION (set (MAP freevars eL)) ∪ {v}’
+    by (‘INFINITE 𝕌(:string)’ by simp [] >>
+        dxrule_then irule $ iffLR NOT_IN_FINITE >>
+        gvs [NOT_IN_FINITE, FINITE_BIGUNION, MEM_MAP] >> rw [] >> fs [freevars_FINITE]) >>
+  irule exp_eq_in_ctxt_trans >> irule_at Any exp_eq_in_ctxt_Apps >>
+  qexists_tac ‘MAP (λe. Let s (Var v) e) (MAP (λe. Let v (Var s) e) eL)’ >>
+  qexists_tac ‘(Let s (Var v) (Let v e e2))’ >>
+  conj_asm1_tac
+  >- (rw [LIST_REL_EL_EQN, EL_MAP] >>
+      irule exp_eq_IMP_exp_eq_in_ctxt >> irule $ iffLR exp_eq_sym >>
+      irule Let_Let_nothing >> gvs [] >>
+      rename1 ‘EL n eL’ >> first_x_assum $ qspecl_then [‘freevars (EL n eL)’] assume_tac >>
+      gvs [MEM_MAP] >> pop_assum $ qspecl_then [‘EL n eL’] assume_tac >> gvs [MEM_EL]) >>
+  conj_asm1_tac
+  >- (irule exp_eq_IMP_exp_eq_in_ctxt >> irule $ iffLR exp_eq_sym >> irule eval_IMP_exp_eq >>
+      rw [Ntimes subst_def 2] >>
+      rename1 ‘subst (f \\ _ )’ >> qspecl_then [‘f’, ‘Let v e e2’] assume_tac $ GSYM subst_fdomsub >>
+      gvs [eval_thm, bind1_def, subst1_ignore, IMP_closed_subst, FRANGE_FLOOKUP]) >>
+  irule exp_eq_in_ctxt_trans >> irule_at (Pos hd) $ iffLR exp_eq_in_ctxt_sym >>
+  irule_at Any Let_Apps_in_ctxt >>
 QED
-        
+
 Theorem find_soundness_lemma:
   ∀e c fdc ds e' fd. find e c fdc ds e' fd
     ⇒ (∀n l i. (n, l) ∈ fdc ∧ i < LENGTH l ∧ EL i l ⇒ (Var n) fdemands (([], i), LENGTH l, c))
@@ -1876,14 +2931,15 @@ Proof
       \\ first_x_assum $ dxrule_then assume_tac
       \\ gvs [Apps_demands, LIST_REL_EL_EQN]
       \\ last_x_assum $ drule_then assume_tac
-      \\ gvs [EL_ZIP, fdemands_def]
+      \\ gvs [EL_ZIP]
       \\ rename1 ‘Apps _ _ demands (d, _)’ \\ PairCases_on ‘d’
       \\ once_rewrite_tac [GSYM needs_Var_is_demands]
       \\ irule needs_trans \\ irule_at (Pos hd) needs_exp_eq
       \\ irule_at Any exp_eq_in_ctxt_Apps
       \\ irule_at Any exp_eq_in_ctxt_l_refl
-      \\ last_x_assum $ irule_at Any
-      \\ first_x_assum $ irule_at Any
+      \\ last_x_assum $ dxrule_then assume_tac \\ gvs []
+      \\ dxrule_then assume_tac fdemands_alt \\ fs []
+      \\ rpt $ first_x_assum $ irule_at Any
       \\ gvs [exp_eq_in_ctxt_sym, needs_Var_is_demands])
   >~[‘exp_eq_in_ctxt c (Proj n i e) (Proj n i e')’] (* find_Proj *)
   >- (strip_tac
@@ -1941,7 +2997,7 @@ Proof
       \\ first_x_assum $ dxrule_then assume_tac
       \\ pop_assum $ qspecl_then [‘e’] assume_tac
       \\ last_x_assum $ dxrule_then assume_tac
-      \\ last_x_assum $ dxrule_then assume_tac \\ fs []
+      \\ last_x_assum $ dxrule_then assume_tac \\ fs [fdemands_def]
       >- (irule exp_eq_in_ctxt_trans \\ first_x_assum $ irule_at Any
           \\ gvs [exp_eq_in_ctxt_App, exp_eq_in_ctxt_refl])
       >~[‘Let _ _ _ demands (d, c)’]
@@ -1950,13 +3006,13 @@ Proof
           \\ ‘d1 = v ∨ d1 ≠ v’ by fs []
           \\ gvs [])
       >~[‘Let _ _ _ fdemands _’]
-      >- (irule fdemands_exp_eq \\ irule_at Any fdemands_Let
+      >- (irule fdemands_exp_eq
           \\ first_x_assum $ irule_at (Pos hd)
           \\ gvs [exp_eq_in_ctxt_refl, exp_eq_in_ctxt_App])
-      \\ irule exp_eq_same_demands \\ irule_at Any demands_Apps2
+      \\ irule exp_eq_same_demands
       \\ irule_at Any exp_eq_in_ctxt_Apps \\ irule_at Any exp_eq_in_ctxt_l_refl
       \\ irule_at Any exp_eq_in_ctxt_App \\ irule_at (Pos hd) exp_eq_in_ctxt_refl
-      \\ first_assum $ irule_at (Pos hd)
+      \\ first_assum $ irule_at (Pos hd) \\ irule_at Any demands_Apps2
       \\ rename1 ‘SND d2’ \\ PairCases_on ‘d2’
       \\ gvs [dest_fd_SND_def] \\ strip_tac
       \\ gvs [])
@@ -1977,16 +3033,16 @@ Proof
           \\ first_x_assum $ irule_at Any
           \\ fs [exp_eq_in_ctxt_App, exp_eq_in_ctxt_refl])
       >~[‘Let _ _ _ fdemands _’]
-      >- (irule fdemands_exp_eq \\ irule_at Any fdemands_Let
+      >- (irule fdemands_exp_eq \\ fs [fdemands_def]
           \\ first_x_assum $ irule_at (Pos hd)
           \\ gvs [exp_eq_in_ctxt_refl, exp_eq_in_ctxt_App])
       >~[‘Let _ _ _ demands (d, c)’]
       >- (rename1 ‘_ demands (d, c)’ \\ PairCases_on ‘d’
-      \\ last_x_assum $ dxrule_then assume_tac
-      \\ fs [demands_Let2]
-      \\ irule demands_Let1
-      \\ first_x_assum $ drule_then assume_tac
-      \\ dxrule_then assume_tac demands_empty_proj \\ fs [])
+          \\ last_x_assum $ dxrule_then assume_tac
+          \\ fs [demands_Let2]
+          \\ irule demands_Let1
+          \\ first_x_assum $ drule_then assume_tac
+          \\ dxrule_then assume_tac demands_empty_proj \\ fs [])
       \\ irule exp_eq_same_demands \\ irule_at Any demands_Apps2
       \\ irule_at Any exp_eq_in_ctxt_Apps \\ irule_at Any exp_eq_in_ctxt_l_refl
       \\ irule_at Any exp_eq_in_ctxt_App \\ irule_at (Pos hd) exp_eq_in_ctxt_refl
